Updates to organization, setting up for a blogpost

Natural_Deduction.v
@@ -1,55 +1,13 @@
 (*Natural deduction formalisation*)
-
-Set Warnings "-notation-overridden,-parsing".
-From Coq Require Import List.
 From Coq Require Import Lists.ListSet.
 From Coq Require Import Arith.PeanoNat.
-
+From Coq Require Import List.
 Import ListNotations.
+From LogicPlayground Require Import Bool_terms.
+
 
 Create HintDb NDhints.
 
-Module Nat_Deduct_Playground.
-Inductive tm : Set :=
-| tTrue  : tm 
-| tFalse : tm
-| tVar   : nat -> tm
-(* | tNot   : tm -> tm *)
-| tAnd   : tm -> tm -> tm
-| tOr    : tm -> tm -> tm
-| tImpl  : tm -> tm -> tm.
-(*  *)
-
- Notation " ⊤ " := tTrue (at level 0).
- Notation " ⊥ " := tFalse (at level 0).
-
- (* Notation " ! A " := (tImpl A tFalse) (at level 75). *)
- Notation " ¬ A " := (tImpl A tFalse) (at level 75).
-
- Notation "A '&&&' B" := (tAnd A B) (at level 80, right associativity). 
- Notation "A '|||' B" := (tOr A B) (at level 85, right associativity).
- Notation "A '-->' B" := (tImpl A B)  (at level 30, right associativity).
-
-Definition context := (list tm)%type.
-
-
-Lemma tm_eq_dec : forall x y:tm, {x=y}+{x<>y}.
-Proof.
-    induction x; destruct y; try (now right); try (now left).
-    - destruct (Nat.eq_dec n n0) eqn:E; subst; auto. right. congruence.
-    - destruct (IHx1 y1) eqn:E1.
-        + destruct (IHx2 y2) eqn:E2; subst; auto.
-          * right. congruence.
-        + right. congruence.
-    - destruct (IHx1 y1) eqn:E1.
-        + destruct (IHx2 y2) eqn:E2; subst; auto.
-            * right. congruence.
-        + right. congruence.
-    - destruct (IHx1 y1) eqn:E1.
-        + destruct (IHx2 y2) eqn:E2; subst; auto.
-            * right. congruence.
-        + right. congruence.
-Qed.
 Coercion tVar : nat >-> tm.
     
 
@@ -120,17 +78,6 @@ Proof.
 Qed.
 
 
-(*Semantics of tm*)
-Definition assignment := list nat.
-Fixpoint truthAssign (A: assignment) (t:tm) : Prop :=
-    match t with
-    | tTrue       => True
-    | tFalse      => False
-    | tVar n      => In n A
-    | p_1 &&& p_2 => (truthAssign A p_1) /\ (truthAssign A p_2)
-    | p_1 ||| p_2 => (truthAssign A p_1) \/ (truthAssign A p_2)
-    | p_1 --> p_2 => (truthAssign A p_1) -> (truthAssign A p_2)
-    end.
 
 Definition listSat (A:assignment) (c:context) := List.Forall (fun x => truthAssign A x) c.
 
@@ -177,4 +124,3 @@ Proof.
     - sound_help. intros * H_1. apply IHdeductionTree in H_1. destruct H_1.
 Qed.
 
-End Nat_Deduct_Playground.
