Bool_terms.v
@@ -1,0 +1,54 @@
+(*Introduction to propositional logic*)
+From Coq Require Import List.
+Import ListNotations.
+Inductive tm : Set :=
+| tTrue  : tm 
+| tFalse : tm
+| tVar   : nat -> tm
+(* | tNot   : tm -> tm *)
+| tAnd   : tm -> tm -> tm
+| tOr    : tm -> tm -> tm
+| tImpl  : tm -> tm -> tm.
+(*  *)
+
+ Notation " ⊤ " := tTrue (at level 0).
+ Notation " ⊥ " := tFalse (at level 0).
+
+ (* Notation " ! A " := (tImpl A tFalse) (at level 75). *)
+ Notation " ¬ A " := (tImpl A tFalse) (at level 75).
+
+ Notation "A '&&&' B" := (tAnd A B) (at level 80, right associativity). 
+ Notation "A '|||' B" := (tOr A B) (at level 85, right associativity).
+ Notation "A '-->' B" := (tImpl A B)  (at level 30, right associativity).
+
+Definition context := (list tm)%type.
+
+(*Semantics of tm*)
+Definition assignment := list nat.
+Fixpoint truthAssign (A: assignment) (t:tm) : Prop :=
+    match t with
+    | tTrue       => True
+    | tFalse      => False
+    | tVar n      => In n A
+    | p_1 &&& p_2 => (truthAssign A p_1) /\ (truthAssign A p_2)
+    | p_1 ||| p_2 => (truthAssign A p_1) \/ (truthAssign A p_2)
+    | p_1 --> p_2 => (truthAssign A p_1) -> (truthAssign A p_2)
+    end.
+
+Lemma tm_eq_dec : forall x y:tm, {x=y}+{x<>y}.
+Proof.
+    induction x; destruct y; try (now right); try (now left).
+    - destruct (Nat.eq_dec n n0) eqn:E; subst; auto. right. congruence.
+    - destruct (IHx1 y1) eqn:E1.
+        + destruct (IHx2 y2) eqn:E2; subst; auto.
+          * right. congruence.
+        + right. congruence.
+    - destruct (IHx1 y1) eqn:E1.
+        + destruct (IHx2 y2) eqn:E2; subst; auto.
+            * right. congruence.
+        + right. congruence.
+    - destruct (IHx1 y1) eqn:E1.
+        + destruct (IHx2 y2) eqn:E2; subst; auto.
+            * right. congruence.
+        + right. congruence.
+Qed.
